examples/new_echo/NewEchoAll.v
@@ -17,16 +17,13 @@ Set Implicit Arguments.
 
 
 
-
-
-
 Section ECHOIMPL.
 
   Let Σ: GRA.t := GRA.of_list [].
   Local Existing Instance Σ.
 
   Definition echo_impl: ModL.t :=
-    Mod.add_list [Mem; Main; Stack; Echo; Client].
+    Mod.add_list [Mem; Stack; Echo; Main; Client].
 
 End ECHOIMPL.
 
@@ -35,8 +32,27 @@ Definition echo_impl_itr := ModSemL.initial_itr (ModL.enclose echo_impl) None.
 
 
 
+Require Import Mem0 NewStackImp NewEchoImp NewEchoMainImp NewClientImp.
+
+Section ECHOIMP.
+
+  Let Σ: GRA.t := GRA.of_list [].
+  Local Existing Instance Σ.
+
+  Definition echo_imp: ModL.t :=
+    Mod.add_list [Mem; Stack; Echo; EchoMain; Client].
+
+End ECHOIMP.
+
+Definition echo_imp_itr := ModSemL.initial_itr (ModL.enclose echo_imp) None.
+
+
 
 Require Import MemOpen NewStack3A NewEcho1 NewEchoMain0 NewClient0.
+Require Import NewEchoMainImp0proof NewStackImp0proof NewEchoImp0proof NewClientImp0proof NewStack01proof NewStack12proof NewStack23Aproof NewEcho01proof.
+Require Import SimModSem.
+Require Import Mem0Openproof MemOpen0proof.
+Require Import Open.
 
 Section ECHOSPEC.
 
@@ -55,7 +71,7 @@ Section ECHOSPEC.
   Qed.
   Local Existing Instance stkRA_inG.
 
-  Let frds: list string := ["Mem"; "Stack"; "Echo"].
+  Let frds: list string := ["Stack"; "Echo"].
   Definition echo_spec: ModL.t :=
     Mod.add_list [
       Mem0.Mem;
@@ -65,25 +81,73 @@ Section ECHOSPEC.
       Client
       ].
 
+  Lemma refines2_cons mhd0 mhd1 mtl0 mtl1
+        (HD: refines2 [mhd0] [mhd1])
+        (TL: refines2 mtl0 mtl1)
+    :
+      refines2 (mhd0::mtl0) (mhd1::mtl1).
+  Proof.
+  Admitted.
+
+  Lemma refines2_app mhd0 mhd1 mtl0 mtl1
+        (HD: refines2 mhd0 mhd1)
+        (TL: refines2 mtl0 mtl1)
+    :
+      refines2 (mhd0++mtl0) (mhd1++mtl1).
+  Proof.
+  Admitted.
+
+  Section PROOF.
+    Theorem echo_correct:
+      refines echo_imp echo_spec.
+    Proof.
+      unfold echo_imp, echo_spec. transitivity echo_impl.
+      { eapply refines2_pairwise. econs.
+        { ss. }
+        econs.
+        { eapply adequacy_local2. eapply NewStackImp0proof.correct. }
+        econs.
+        { eapply adequacy_local2. eapply NewEchoImp0proof.correct. }
+        econs.
+        { eapply adequacy_local2. eapply NewEchoMainImp0proof.correct. }
+        econs.
+        { eapply adequacy_local2. eapply NewClientImp0proof.correct. }
+        ss.
+      }
+      unfold echo_impl.
+      pose (kmd0 := [KMem; NewStack1.KStack]).
+      transitivity (Mod.add_list (KMod.transl_tgt_list kmd0 ++ [NewEcho0.Echo; NewEchoMain0.Main; Client])).
+      { eapply refines2_cons.
+        { eapply adequacy_local2. eapply Mem0Openproof.correct. }
+        eapply refines2_cons.
+        { eapply adequacy_local2. eapply NewStack01proof.correct. i.
+          etrans; [|eapply to_closed_stb_weaker].
+          stb_incl_tac; tauto. }
+        refl.
+      }
+      etrans.
+      { rewrite Mod.add_list_app. eapply refines_proper_r.
+        eapply adequacy_open. }
+      pose (kmd1 := [NewStack3A.KStack; KEcho]).
+      transitivity (Mod.add_list (Mem0.Mem :: (KMod.transl_tgt_list kmd1) ++ [Main; Client])).
+      { rewrite <- Mod.add_list_app. eapply refines2_cons.
+        { eapply adequacy_local2. eapply MemOpen0proof.correct. }
+        eapply refines2_cons.
+        { etrans.
+          { eapply adequacy_local2. eapply NewStack12proof.correct. }
+          { eapply adequacy_local2. eapply NewStack23Aproof.correct. }
+        }
+        eapply refines2_cons.
+        { eapply adequacy_local2. eapply NewEcho01proof.correct. i.
+          autounfold with stb. admit "stb". }
+        refl.
+      }
+      eapply refines2_cons; [refl|].
+      transitivity (KMod.transl_src_list kmd1 ++ [Main; Client]); [|refl].
+      eapply refines2_app; [|refl].
+      eapply adequacy_open.
+    Qed.
+  End PROOF.
 End ECHOSPEC.
 
 Definition echo_spec_itr := ModSemL.initial_itr (ModL.enclose echo_spec) None.
-
-
-
-
-
-
-Require Import Mem0 NewStackImp NewEchoImp NewEchoMainImp NewClientImp.
-
-Section ECHOIMP.
-
-  Let Σ: GRA.t := GRA.of_list [].
-  Local Existing Instance Σ.
-
-  Definition echo_imp: ModL.t :=
-    Mod.add_list [Mem; EchoMain; Stack; Echo; Client].
-
-End ECHOIMP.
-
-Definition echo_imp_itr := ModSemL.initial_itr (ModL.enclose echo_imp) None.
