examples/new_stack/NewStack3A.v
@@ -123,7 +123,7 @@ Section PROOF.
 
   Definition KStack: KMod.t := {|
     KMod.get_modsem := fun _ => KStackSem;
-    KMod.sk := Sk.unit;
+    KMod.sk := [("new", Sk.Gfun); ("pop", Sk.Gfun); ("push", Sk.Gfun)];
   |}
   .
   Definition Stack (stb: Sk.t -> gname -> option fspec): Mod.t :=
